coq/cclc/clc_subtype.v
@@ -18,7 +18,16 @@ Inductive sub1 : term -> term -> Prop :=
 | sub1_sigma A1 A2 B1 B2 s r t :
   sub1 A1 A2 ->
   sub1 B1 B2 ->
-  sub1 (Sigma A1 B1 s r t) (Sigma A2 B2 s r t).
+  sub1 (Sigma A1 B1 s r t) (Sigma A2 B2 s r t)
+| sub1_inp A B1 B2 s :
+  sub1 B1 B2 ->
+  sub1 (Inp A B1 s) (Inp A B2 s)
+| sub1_out A B1 B2 s :
+  sub1 B1 B2 ->
+  sub1 (Out A B1 s) (Out A B2 s)
+| sub1_ch A1 A2 :
+  sub1 A1 A2 ->
+  sub1 (Ch A1) (Ch A2).
 
 CoInductive sub (A B : term) : Prop :=
 | SubI A' B' : 
@@ -46,28 +55,55 @@ Proof with eauto 6 using sub1, sub1_sub, sub1_conv, conv_sub1.
     [ A C D 
     | s l1 l2 leq C D conv sb
     | A B1 B2 s r t sb1 ih C D conv sb2 
-    | A1 A2 B1 B2 s r t sb1 ih1 sb2 ih2 C D conv sb3 ]...
+    | A1 A2 B1 B2 s r t sb1 ih1 sb2 ih2 C D conv sb3
+    | A B1 B2 s sb1 ih C D conv sb2
+    | A B1 B2 s sb1 ih C D conv sb2
+    | A1 A2 sb1 ih C D conv sb2 ]...
   inv sb; try (exfalso; solve_conv)...
-    move: conv => /sort_inj [->eq].
-    apply: sub_sort. subst.
-    exact: leq_trans leq _.
+    move:conv=>/sort_inj[->eq].
+    apply:sub_sort. subst.
+    exact:leq_trans leq _.
   inv sb2; try (exfalso; solve_conv)...
-    move: conv => /pi_inj[conv1 [conv2[->[->->]]]].
-    move: (ih _ _ conv2 H) => {ih} sub. inv sub.
-    apply: SubI. 
+    move:conv=>/pi_inj[conv1[conv2[->[->->]]]].
+    move:(ih _ _ conv2 H)=>{ih}sub. inv sub.
+    apply:SubI. 
     apply sub1_pi with (s := s0) (r := r0) (t := t0)... 
-    exact: conv_pi. 
-    exact: conv_pi.
+    exact:conv_pi. 
+    exact:conv_pi.
   inv sb3; try (exfalso; solve_conv)...
-    move: conv => /sigma_inj[conv1[conv2[->[->->]]]].
-    move: (ih1 _ _ conv1 H)=>{ih1}sub1.
-    move: (ih2 _ _ conv2 H0)=>{ih2}sub2.
+    move:conv=>/sigma_inj[conv1[conv2[->[->->]]]].
+    move:(ih1 _ _ conv1 H)=>{ih1}sub1.
+    move:(ih2 _ _ conv2 H0)=>{ih2}sub2.
     inv sub1. inv sub2.
-    apply: SubI.
+    apply:SubI.
     apply sub1_sigma with (s := s0) (r := r0) (t := t0).
-    exact: H1. exact: H4.
-    exact: conv_sigma.
-    exact: conv_sigma.
+    exact:H1. exact:H4.
+    exact:conv_sigma.
+    exact:conv_sigma.
+  inv sb2; try (exfalso; solve_conv)...
+    move:conv=>/inp_inj[conv1[conv2->]].
+    move:(ih _ _ conv2 H)=>{ih}sub. inv sub.
+    apply:SubI.
+    apply sub1_inp with (s := s0).
+    exact:H0.
+    exact:conv_inp.
+    exact:conv_inp.
+  inv sb2; try (exfalso; solve_conv)...
+    move:conv=>/out_inj[conv1[conv2->]].
+    move:(ih _ _ conv2 H)=>{ih}sub. inv sub.
+    apply:SubI.
+    apply sub1_out with (s := s0).
+    exact:H0.
+    exact:conv_out.
+    exact:conv_out.
+  inv sb2; try (exfalso; solve_conv)...
+    move:conv=>/ch_inj conv.
+    move:(ih _ _ conv H)=>{ih}sub. inv sub.
+    apply:SubI.
+    apply sub1_ch.
+    exact:H0.
+    exact:conv_ch.
+    exact:conv_ch.
 Qed.
 
 Lemma sub_trans B A C :
@@ -89,6 +125,9 @@ Proof.
   move=> s l0 l3 leq /sort_inj[->->]/sort_inj[<-<-]=> //.
   move=> *. exfalso; solve_conv.
   move=> *. exfalso; solve_conv.
+  move=> *. exfalso; solve_conv.
+  move=> *. exfalso; solve_conv.
+  move=> *. exfalso; solve_conv.
 Qed.
 
 Lemma sub_pi_inv A1 A2 s1 s2 r1 r2 t1 t2 B1 B2 :
@@ -107,6 +146,9 @@ Proof.
     firstorder.
     exact: conv_trans c3. exact: SubI sb c2 c4.
   move=> *. exfalso; solve_conv.
+  move=> *. exfalso; solve_conv.
+  move=> *. exfalso; solve_conv.
+  move=> *. exfalso; solve_conv.
 Qed.
 
 Lemma sub_sigma_inv A1 A2 B1 B2 p1 p2 q1 q2 s1 s2 :
@@ -124,6 +166,69 @@ Proof.
   move=>A A0 B0 B3 s r t sb1 sb2
     /sigma_inj[c1[c2[<-[<-<-]]]]/sigma_inj[c3 [c4 [->[->->]]]]. 
     firstorder. exact: SubI sb1 c1 c3. exact: SubI sb2 c2 c4.
+  move=> *. exfalso; solve_conv.
+  move=> *. exfalso; solve_conv.
+  move=> *. exfalso; solve_conv.
+Qed.
+
+Lemma sub_inp_inv A1 A2 B1 B2 s1 s2 :
+  Inp A1 B1 s1 <: Inp A2 B2 s2 -> 
+  A1 === A2 /\ B1 <: B2 /\ s1 = s2.
+Proof.
+  move=> [A' B' []].
+  move=> C c1 c2. 
+    have{c1 c2}/inp_inj[c1[c2->]]: 
+      Inp A1 B1 s1 === Inp A2 B2 s2.
+    exact: conv_trans c2.
+    firstorder=>//. exact: conv_sub.
+  move=> *. exfalso; solve_conv.
+  move=> *. exfalso; solve_conv.
+  move=> *. exfalso; solve_conv.
+  move=> A B0 B3 s sb 
+    /inp_inj[c1[c2<-]]/inp_inj[c3[c4->]]. 
+    firstorder.
+    exact: conv_trans c3. exact: SubI sb c2 c4.
+  move=> *. exfalso; solve_conv.
+  move=> *. exfalso; solve_conv.
+Qed.
+
+Lemma sub_out_inv A1 A2 B1 B2 s1 s2 :
+  Out A1 B1 s1 <: Out A2 B2 s2 -> 
+  A1 === A2 /\ B1 <: B2 /\ s1 = s2.
+Proof.
+  move=> [A' B' []].
+  move=> C c1 c2. 
+    have{c1 c2}/out_inj[c1[c2->]]: 
+      Out A1 B1 s1 === Out A2 B2 s2.
+    exact: conv_trans c2.
+    firstorder=>//. exact: conv_sub.
+  move=> *. exfalso; solve_conv.
+  move=> *. exfalso; solve_conv.
+  move=> *. exfalso; solve_conv.
+  move=> *. exfalso; solve_conv.
+  move=> A B0 B3 s sb 
+    /out_inj[c1[c2<-]]/out_inj[c3[c4->]]. 
+    firstorder.
+    exact: conv_trans c3. exact: SubI sb c2 c4.
+  move=> *. exfalso; solve_conv.
+Qed.
+
+Lemma sub_ch_inv A1 A2 :
+  Ch A1 <: Ch A2 -> A1 <: A2.
+Proof.
+  move=> [A' B' []].
+  move=> C c1 c2. 
+    have{c1 c2}/ch_inj c1: 
+      Ch A1 === Ch A2.
+    exact: conv_trans c2.
+    firstorder=>//. exact: conv_sub.
+  move=> *. exfalso; solve_conv.
+  move=> *. exfalso; solve_conv.
+  move=> *. exfalso; solve_conv.
+  move=> *. exfalso; solve_conv.
+  move=> *. exfalso; solve_conv.
+  move=>A A3 sb /ch_inj c1/ch_inj c2.
+  exact: SubI sb c1 c2.
 Qed.
 
 Lemma sub1_subst σ A B : sub1 A B -> sub1 A.[σ] B.[σ].
